extracted_code/Z3Solver.ml
@@ -18,6 +18,7 @@ let rec z3_expr_from_coq_smt_bool_expr (expr : SmtExpr.coq_SmtBoolExpr) (ctx : Z
   | SmtExpr.SmtBoolOr (e1, e2) -> Z3.Boolean.mk_or ctx [z3_expr_from_coq_smt_bool_expr e1 ctx vars; z3_expr_from_coq_smt_bool_expr e2 ctx vars]
   | SmtExpr.SmtBoolNot e -> Z3.Boolean.mk_not ctx (z3_expr_from_coq_smt_bool_expr e ctx vars)
   | SmtExpr.SmtBoolEq (a1, a2) -> Z3.Boolean.mk_eq ctx (z3_expr_from_coq_smt_arith_expr a1 ctx vars) (z3_expr_from_coq_smt_arith_expr a2 ctx vars)
+  | SmtExpr.SmtBoolLt (a1, a2) -> Z3.BitVector.mk_ult ctx (z3_expr_from_coq_smt_arith_expr a1 ctx vars) (z3_expr_from_coq_smt_arith_expr a2 ctx vars)
 and z3_expr_from_coq_smt_arith_expr (expr : SmtExpr.coq_SmtArithExpr) (ctx : Z3.context) (vars : var_tracker)
   : Z3.Expr.expr =
   match expr with
