CrSymbolicSemanticsTransformer.v
@@ -61,14 +61,22 @@ Definition eval_hdr_op_assign_smt (ho : HdrOp) (ps: SymbolicState) : SymbolicSta
 Definition eval_hdr_op_list_smt (hol : list HdrOp) (ps : SymbolicState) : SymbolicState :=
   List.fold_left (fun acc op => eval_hdr_op_assign_smt op acc) hol ps.
 
+Definition eval_cmp_smt (op : CmpOp) (e1 e2 : SmtArithExpr) : SmtBoolExpr :=
+  match op with
+  | CmpEq => SmtBoolEq e1 e2
+  | CmpGt => SmtBoolLt e2 e1
+  | CmpLt => SmtBoolLt e1 e2
+  end.
+
 Definition eval_match_smt (match_pattern : MatchPattern) (ps : SymbolicState) : SmtBoolExpr :=
   (* For every list element, check if the Header's current value (determined by ps) equals the uint8 *)
   (* Note that because SmtBoolAnd is associative and commutative, both fold_left and fold_right give the same answer. *)
-  List.fold_right (fun '(h, v) acc =>
-    match acc with
-    | SmtTrue => SmtBoolEq (lookup_varlike ps h) (SmtArithConst v)
-    | _ => SmtBoolAnd (SmtBoolEq (lookup_varlike ps h) (SmtArithConst v)) acc
-    end) SmtTrue match_pattern.
+  List.fold_right (fun '(h, c, v) acc =>
+    let v' := match v with
+    | MatchConst k' => SmtArithConst k'
+    | MatchHeader h' => lookup_varlike ps h'
+    end in
+    SmtBoolAnd (eval_cmp_smt c (lookup_varlike ps h) v') acc) SmtTrue match_pattern.
 
 (* Maybe there's an intermediate function that evaluates a *single* HdrOp conditionally? *)
 Definition eval_hdr_op_assign_smt_conditional
@@ -92,7 +100,6 @@ Definition eval_hdr_op_assign_smt_conditional
 Definition eval_seq_rule_smt (srule : SeqRule) (ps : SymbolicState) : (SymbolicState) :=
   match srule with
   | SeqCtr match_pattern action =>
-        (* First evaluate the match pattern by itself against the original state ps *)
         let condition := eval_match_smt match_pattern ps in
 
         (* Second, evaluate all the hdr_ops contained in the action to get a new intermediate state ps' from ps *)
@@ -145,10 +152,10 @@ Fixpoint switch_case_expr (cases : list (SmtBoolExpr * SmtArithExpr)) (default_c
 (* Compute match results for each match pattern (one embedded in each rule) *)
 Definition get_match_results_smt (t : Transformer) (ps : SymbolicState) : list SmtBoolExpr :=
   List.map (fun rule =>
-                       match rule with 
-                        | Seq (SeqCtr match_pattern _) => eval_match_smt match_pattern ps
-                        | Par (ParCtr match_pattern _) => eval_match_smt match_pattern ps
-                       end) t.
+    match rule with
+    | Seq (SeqCtr match_pattern _) => eval_match_smt match_pattern ps
+    | Par (ParCtr match_pattern _) => eval_match_smt match_pattern ps
+    end) t.
 
 Definition eval_transformer_smt (t : Transformer) (ps : SymbolicState) : SymbolicState :=
   (* get all future program states, one for each rule *)
