ConcreteTransformerLemmas.v
@@ -1,0 +1,211 @@
+From MyProject Require Import CrIdentifiers.
+From MyProject Require Import CrVal.
+From MyProject Require Import CrTransformer.
+From MyProject Require Import CrProgramState.
+From MyProject Require Import CrVarLike.
+From MyProject Require Import CrConcreteSemanticsTransformer.
+From MyProject Require Import PMapHelperLemmas.
+From MyProject Require Import ListUtils.
+From MyProject Require Import Maps.
+From Stdlib Require Import Lists.List.
+From Stdlib Require Import PArith.BinPos.
+Import ListNotations.
+
+(* The convenient equivalence: c1 and c2 agree on every program-variable
+   lookup. *)
+Definition cs_lookup_eq (c1 c2 : ConcreteState) : Prop :=
+  (forall h : Header, lookup_varlike c1 h = lookup_varlike c2 h) /\
+  (forall s : State,  lookup_varlike c1 s = lookup_varlike c2 s) /\
+  (forall c : Ctrl,   lookup_varlike c1 c = lookup_varlike c2 c).
+
+Transparent lookup_varlike_map.
+Transparent map_from_ps.
+Transparent update_varlike.
+Transparent lookup_varlike.
+
+(* update_varlike preserves cs_lookup_eq, regardless of the variable type.
+
+   The cross-type cases (e.g. updating a Header doesn't affect State / Ctrl
+   lookups) are definitional, so [apply ...] discharges them directly. *)
+Lemma cs_lookup_eq_update_header :
+  forall c1 c2 (h : Header) (x : CrVal),
+  cs_lookup_eq c1 c2 ->
+  cs_lookup_eq (update_varlike c1 h x) (update_varlike c2 h x).
+Proof.
+  intros c1 c2 h x [Hh [Hs Hc]].
+  split; [| split].
+  - intros h'. rewrite ! lookup_update_header_header.
+    destruct h, h'. destruct (Coqlib.peq _ _); auto.
+  - apply Hs.
+  - apply Hc.
+Qed.
+
+Lemma cs_lookup_eq_update_state :
+  forall c1 c2 (s : State) (x : CrVal),
+  cs_lookup_eq c1 c2 ->
+  cs_lookup_eq (update_varlike c1 s x) (update_varlike c2 s x).
+Proof.
+  intros c1 c2 s x [Hh [Hs' Hc]].
+  split; [| split].
+  - apply Hh.
+  - intros s'. rewrite ! lookup_update_state_state.
+    destruct s, s'. destruct (Coqlib.peq _ _); auto.
+  - apply Hc.
+Qed.
+
+Lemma cs_lookup_eq_update_ctrl :
+  forall c1 c2 (c : Ctrl) (x : CrVal),
+  cs_lookup_eq c1 c2 ->
+  cs_lookup_eq (update_varlike c1 c x) (update_varlike c2 c x).
+Proof.
+  intros c1 c2 c x [Hh [Hs Hc']].
+  split; [| split].
+  - apply Hh.
+  - apply Hs.
+  - intros c'. rewrite ! lookup_update_ctrl_ctrl.
+    destruct c, c'. destruct (Coqlib.peq _ _); auto.
+Qed.
+
+(* lookup_concrete (used to evaluate function arguments) commutes with
+   cs_lookup_eq. *)
+Lemma lookup_concrete_eq :
+  forall c1 c2 arg,
+  cs_lookup_eq c1 c2 ->
+  lookup_concrete arg c1 = lookup_concrete arg c2.
+Proof.
+  intros c1 c2 arg [Hh [Hs Hc]]. destruct arg; simpl;
+    [apply Hc | apply Hh | reflexivity | apply Hs].
+Qed.
+
+Lemma eval_hdr_op_expr_concrete_eq :
+  forall c1 c2 op,
+  cs_lookup_eq c1 c2 ->
+  eval_hdr_op_expr_concrete op c1 = eval_hdr_op_expr_concrete op c2.
+Proof.
+  intros c1 c2 op Hcs.
+  destruct op; simpl;
+    rewrite (lookup_concrete_eq _ _ arg1 Hcs);
+    rewrite (lookup_concrete_eq _ _ arg2 Hcs);
+    reflexivity.
+Qed.
+
+Lemma eval_match_concrete_eq :
+  forall c1 c2 mp,
+  cs_lookup_eq c1 c2 ->
+  eval_match_concrete mp c1 = eval_match_concrete mp c2.
+Proof.
+  intros c1 c2 mp [Hh [Hs Hc]].
+  unfold eval_match_concrete.
+  induction mp as [|[[hh cmp] mv] rest IH]; simpl; auto.
+  rewrite IH. f_equal. f_equal.
+  - apply Hh.
+  - destruct mv; [reflexivity | apply Hh].
+Qed.
+
+Lemma eval_hdr_op_assign_concrete_preserves_eq :
+  forall c1 c2 op,
+  cs_lookup_eq c1 c2 ->
+  cs_lookup_eq (eval_hdr_op_assign_concrete op c1) (eval_hdr_op_assign_concrete op c2).
+Proof.
+  intros c1 c2 op Hcs.
+  pose proof (eval_hdr_op_expr_concrete_eq c1 c2 op Hcs) as Hexp.
+  unfold eval_hdr_op_assign_concrete.
+  destruct op as [f arg1 arg2 target | f arg1 arg2 target]; rewrite Hexp.
+  - apply cs_lookup_eq_update_state. assumption.
+  - apply cs_lookup_eq_update_header. assumption.
+Qed.
+
+Lemma eval_hdr_op_list_concrete_preserves_eq :
+  forall c1 c2 hol,
+  cs_lookup_eq c1 c2 ->
+  cs_lookup_eq (eval_hdr_op_list_concrete hol c1) (eval_hdr_op_list_concrete hol c2).
+Proof.
+  intros c1 c2 hol. revert c1 c2.
+  induction hol as [|op rest IH]; intros.
+  - simpl. assumption.
+  - simpl. apply IH. apply eval_hdr_op_assign_concrete_preserves_eq. assumption.
+Qed.
+
+Lemma eval_seq_rule_concrete_preserves_eq :
+  forall c1 c2 sr,
+  cs_lookup_eq c1 c2 ->
+  cs_lookup_eq (eval_seq_rule_concrete sr c1) (eval_seq_rule_concrete sr c2).
+Proof.
+  intros c1 c2 [mp action] Hcs. simpl.
+  rewrite (eval_match_concrete_eq _ _ mp Hcs).
+  destruct (eval_match_concrete mp c2); auto.
+  apply eval_hdr_op_list_concrete_preserves_eq. assumption.
+Qed.
+
+Lemma eval_par_rule_concrete_preserves_eq :
+  forall c1 c2 pr,
+  cs_lookup_eq c1 c2 ->
+  cs_lookup_eq (eval_par_rule_concrete pr c1) (eval_par_rule_concrete pr c2).
+Proof.
+  intros c1 c2 [mp action] Hcs. simpl.
+  rewrite (eval_match_concrete_eq _ _ mp Hcs).
+  destruct (eval_match_concrete mp c2); auto.
+  apply eval_hdr_op_list_concrete_preserves_eq. assumption.
+Qed.
+
+Lemma eval_match_action_rule_concrete_preserves_eq :
+  forall c1 c2 rule,
+  cs_lookup_eq c1 c2 ->
+  cs_lookup_eq (eval_match_action_rule_concrete rule c1) (eval_match_action_rule_concrete rule c2).
+Proof.
+  intros c1 c2 [sr | pr] Hcs.
+  - apply eval_seq_rule_concrete_preserves_eq. assumption.
+  - apply eval_par_rule_concrete_preserves_eq. assumption.
+Qed.
+
+Lemma get_match_results_eq :
+  forall c1 c2 t,
+  cs_lookup_eq c1 c2 ->
+  get_match_results t c1 = get_match_results t c2.
+Proof.
+  intros c1 c2 t Hcs.
+  unfold get_match_results.
+  apply map_ext. intros [[mp _] | [mp _]]; apply eval_match_concrete_eq; assumption.
+Qed.
+
+Lemma eval_transformer_concrete_preserves_eq :
+  forall c1 c2 t,
+  cs_lookup_eq c1 c2 ->
+  cs_lookup_eq (eval_transformer_concrete t c1) (eval_transformer_concrete t c2).
+Proof.
+  intros c1 c2 t Hcs.
+  unfold eval_transformer_concrete.
+  rewrite (get_match_results_eq _ _ t Hcs).
+  destruct (find_first_match (combine (get_match_results t c2) t)) as [rule|]; auto.
+  apply eval_match_action_rule_concrete_preserves_eq. assumption.
+Qed.
+
+(* Convenient repackaged form: agreement at all 3 varlike types is preserved
+   pointwise by the transformer. *)
+Lemma transformer_preserves_lookup_equality_lemma :
+  forall t c1 c2,
+  (forall (h : Header) (s : State) (c : Ctrl),
+    lookup_varlike c1 h = lookup_varlike c2 h /\
+    lookup_varlike c1 s = lookup_varlike c2 s /\
+    lookup_varlike c1 c = lookup_varlike c2 c)
+  ->
+  (forall (h : Header) (s : State) (c : Ctrl),
+    lookup_varlike (eval_transformer_concrete t c1) h = lookup_varlike (eval_transformer_concrete t c2) h /\
+    lookup_varlike (eval_transformer_concrete t c1) s = lookup_varlike (eval_transformer_concrete t c2) s /\
+    lookup_varlike (eval_transformer_concrete t c1) c = lookup_varlike (eval_transformer_concrete t c2) c).
+Proof.
+  intros t c1 c2 H.
+  assert (Hcs : cs_lookup_eq c1 c2).
+  { split; [| split].
+    - intros v. apply (H v (StateCtr xH) (CtrlCtr xH)).
+    - intros v. apply (H (HeaderCtr xH) v (CtrlCtr xH)).
+    - intros v. apply (H (HeaderCtr xH) (StateCtr xH) v). }
+  pose proof (eval_transformer_concrete_preserves_eq _ _ t Hcs) as [Hh' [Hs' Hc']].
+  intros h s c. split; [| split].
+  - apply Hh'.
+  - apply Hs'.
+  - apply Hc'.
+Qed.
+
+Global Opaque lookup_varlike_map.
+Global Opaque map_from_ps.
