CtrlPlaneInvariants.v
@@ -4,6 +4,7 @@ From MyProject Require Import CrConcreteSemanticsTransformer.
 From MyProject Require Import CrProgramState.
 From MyProject Require Import ListUtils.
 From Stdlib Require Import Lists.List.
+From Stdlib Require Import Bool.Bool.
 
 (* Effectively, ctrl plane doesn't change *)
 Lemma ctrl_plane_invariant_hdr_op:
