SmtModuleQuery.v
@@ -1,0 +1,96 @@
+From Stdlib Require Import ZArith.
+From Stdlib Require Import String.
+From Stdlib Require Import List.
+Import ListNotations.
+From MyProject Require Import Maps.
+From MyProject Require Import SmtTypes.
+From MyProject Require Import SmtExpr.
+From MyProject Require Import SmtQuery.
+From MyProject Require Import CrIdentifiers.
+From MyProject Require Import CrVarLike.
+From MyProject Require Import CrModule.
+From MyProject Require Import CrProgramState.
+From MyProject Require Import CrDslProperties.
+From MyProject Require Import CrTModSymbolicSemantics.
+From MyProject Require Import CrTModConcreteSemantics.
+
+Definition keys_from_map {T A : Type} (fn : positive -> A) (m : PMap.t T) : list A :=
+  List.map fn (List.map fst (PTree.elements (snd m))).
+
+Definition modnet_equivalence_checker
+  (p1 : GeneralCaracaraProgram) (p2 : GeneralCaracaraProgram)
+  : EquivalenceResult :=
+  let sym1_opt := eval_general_program_symbolic_sinks p1 (init_general_symbolic_state "p1" p1) in
+  let sym2_opt := eval_general_program_symbolic_sinks p2 (init_general_symbolic_state "p2" p2) in
+  match sym1_opt, sym2_opt with
+  | Some [sym1], Some [sym2] => (* assume one sink *)
+    let h_map : PMap.t SmtArithExpr := (header_map sym1) in
+    let header_ids : list Header := get_signature_from_general p1 in
+    match smt_query (check_headers_and_state_vars sym1 sym2 header_ids []) with
+    | SmtUnsat => Equivalent
+    | SmtSat f => NotEquivalent f
+    | SmtUnknown => NotEquivalentUnknown
+    end
+  | _, _ => NotEquivalentVariablesDiffer
+  end.
+
+Definition is_linear_chain (p : GeneralCaracaraProgram) : Prop :=
+  let net := get_network_from_general p in
+  is_dag net /\
+  single_sink net /\
+  no_fan_out net /\
+  no_fan_in net.
+
+(* NOTE/TODO: Open question about state equivalence and what it means for states to be equivalent for different network topologies *)
+Lemma modnet_equivalence_checker_sound :
+  forall p1 p2 f,
+  (* if two programs *)
+  well_formed_general_program p1 ->
+  well_formed_general_program p2 ->
+  (* have a single source and sink *)
+  is_linear_chain p1 ->
+  is_linear_chain p2 ->
+  (* if they're considered equivalent *)
+  modnet_equivalence_checker p1 p2 = Equivalent ->
+  (* then when starting from their initial concrete states *)
+  let ci_1 := concretize_sym_modnet_state (init_general_symbolic_state "p1" p1) f in
+  let ci_2 := concretize_sym_modnet_state (init_general_symbolic_state "p2" p2) f in
+  (* they each produce a single final state *)
+  let opt_cf_1_l := eval_general_program_concrete_sinks p1 ci_1 in
+  let opt_cf_2_l := eval_general_program_concrete_sinks p2 ci_2 in
+  exists cf_1 cf_2,
+  opt_cf_1_l = Some [cf_1] /\
+  opt_cf_2_l = Some [cf_2] /\
+  (* in which the output headers are identical *)
+  (forall h, In h (get_headers_from_general p1) ->
+    lookup_varlike cf_1 h = lookup_varlike cf_2 h).
+Proof.
+Admitted.
+
+Lemma modnet_equivalence_checker_complete :
+  forall p1 p2 f,
+  (* if two programs *)
+  well_formed_general_program p1 ->
+  well_formed_general_program p2 ->
+  (* have a single source and sink *)
+  is_linear_chain p1 ->
+  is_linear_chain p2 ->
+  (* if they're not considered equivalent *)
+  modnet_equivalence_checker p1 p2 = NotEquivalent f ->
+  (* then when starting from their initial concrete states *)
+  let ci_1 := concretize_sym_modnet_state (init_general_symbolic_state "p1" p1) f in
+  let ci_2 := concretize_sym_modnet_state (init_general_symbolic_state "p2" p2) f in
+  (* they each produce a single final state *)
+  let opt_cf_1_l := eval_general_program_concrete_sinks p1 ci_1 in
+  let opt_cf_2_l := eval_general_program_concrete_sinks p2 ci_2 in
+  exists cf_1 cf_2,
+  opt_cf_1_l = Some [cf_1] /\
+  opt_cf_2_l = Some [cf_2] /\
+  (* in which the output headers differ on at least one header *)
+  (exists h, In h (get_signature_from_general p1) /\
+    lookup_varlike cf_1 h <> lookup_varlike cf_2 h).
+Proof.
+Admitted.
+
+Print Assumptions modnet_equivalence_checker_sound.
+Print Assumptions modnet_equivalence_checker_complete.
